On utilise la formule de dérivation d'un produit : $(uv)' = u'v + uv'$

Posons :
- $u(x) = \ln(x^2 + 1)$
- $v(x) = e^{2x}$

**Calcul de $u'(x)$ :**

$$u'(x) = \frac{(x^2 + 1)'}{x^2 + 1} = \frac{2x}{x^2 + 1}$$

**Calcul de $v'(x)$ :**

$$v'(x) = 2e^{2x}$$

**Application de la formule du produit :**

$$f'(x) = u'(x) \cdot v(x) + u(x) \cdot v'(x)$$

$$f'(x) = \frac{2x}{x^2 + 1} \cdot e^{2x} + \ln(x^2 + 1) \cdot 2e^{2x}$$

$$f'(x) = e^{2x} \left( \frac{2x}{x^2 + 1} + 2\ln(x^2 + 1) \right)$$

**Réponse :**

$$f'(x) = 2e^{2x} \left( \frac{x}{x^2 + 1} + \ln(x^2 + 1) \right)$$
